\input{macros.tex}

\author{
    Marc \textsc{Chevalier}\\
    Thomas \textsc{Pellissier} \textsc{Tanon}}
\date{\today}
\title{\textsc{Friedman}'s translation}

\begin{document}

\maketitle

\section{\textsc{Friedman}'s Translation}

\begin{definition}
    Let $\R$ be a formula. The \textbf{parametrized negation} is 
    $$
        \neg_\R := A \Rightarrow \R
    $$
\end{definition}

We gather here some basic properties of the parametrized negation

\begin{proposition}
    In intuitionisctic logic,
    \begin{enumerate}[(i)]
        \item $B \Rightarrow \neg_\R A \vdash A \Rightarrow \neg_\R B$
        \item $A\vdash \neg_\R\neg_\R A$
        \item $A\Rightarrow B \vdash \neg_\R B \Rightarrow \neg_\R A$
        \item $A\Rightarrow B \vdash \neg_\R\neg_\R A \Rightarrow \neg_\R \neg_\R B$
        \item $\neg_\R \neg_\R \neg_\R A \vdash \neg_\R A$
    \end{enumerate}
\end{proposition}
\begin{proof}
    \input{src/prop1-2.tex}
\end{proof}

We now define the parametrized translation.
\begin{definition}
    Let $\R$ be a formula. The \textbf{parametrized negative translation} $A^{\neg_\R}$ is defined by induction on $A$ as follows:
    \begin{center}
    \begin{tabular}{cccc}
        $\bottom^{\neg_\R} := \R$ & $\top^{\neg_\R} := \top$ & \multicolumn{2}{c}{$(a\dot{=}b)^{\neg_\R} := \neg_\R\neg_\R(a\dot{=}b)$}\\
        \multicolumn{2}{c}{$(A\wedge B)^{\neg_R}:=A^{\neg_\R} \wedge B^{\neg_\R}$} & \multicolumn{2}{c}{$(A \Rightarrow B)^{\neg_R}:=A^{\neg_\R} \Rightarrow B^{\neg_\R}$}\\
        \multicolumn{4}{c}{$(A \vee B)^{\neg_R}:=\neg_\R\neg_\R(A^{\neg_\R} \vee B^{\neg_\R})$}\\
        \multicolumn{2}{c}{$\forall x A)^{\neg_\R} := \forall x A^{\neg_\R}$} & \multicolumn{2}{c}{$\exists x A^{\neg_\R} := \neg_\R\neg_\R(\exists x A^{\neg_\R})$}
    \end{tabular}
    \end{center}
\end{definition}

Note that $(\neg A)^{\neg_\R} = \neg_\R A^{\neg_\R}$. We gather here the basic properties of the parametrized translation.

\begin{proposition}
    In intuitionistic logic,
    \begin{enumerate}[(i)]
        \item $\vdash (A\vee \neg A)^{\neg_\R}$
        \item $\R \vdash A^{\neg_\R}$
        \item $\neg_\R\neg_\R A^{\neg_\R} \vdash A^{\neg_\R}$
    \end{enumerate}
\end{proposition}
\begin{proof}
    \input{src/prop1-4.tex}
\end{proof}


\end{document}