\begin{enumerate}[(i)]
    \item We proof this property by induction.
    We will use intensively these lemmas:
    $$
    \infer{
        (\Psi_1) : \neg A \vdash \neg_\R A
    }{
        \infer{
            \neg A, A \vdash \R
        }{
            \infer{
                \neg A, A \vdash \bot
            }{
                \infer{
                    \neg A, A \vdash \neg A
                }{
                }&
                \infer{
                    \neg A, A \vdash A
                }{
                }
            }
        }
    }
    $$
    
    $$
    \infer{
        (\Psi_2) : A \vdash \neg_\R \neg_\R A
    }{
        \infer{
            A, \neg_\R A \vdash \R
        }{
            \infer{
                A, \neg_\R A \vdash A\Rightarrow \R
            }{
            }&
            \infer{
                A, \neg_\R A \vdash A
            }{
            }
        }
    }
    $$
    
    $$
    \infer{
        (\Psi_3) :\: \vdash \neg_\R \neg_\R A
    }{
        \infer{
             \neg_\R A \vdash \R
        }{
            \infer{
                 \neg_\R A \vdash A\Rightarrow \R
            }{
            }&
            \neg_\R A \vdash A
        }
    }
    $$
    
    We will often use this last one with the weakening
    
    \begin{itemize}
        \item $A = \top$.
            $$
            \infer{
                \vdash (\top \vee \neg \top)^{\neg_\R}
            }{
                \infer{
                    \vdash (\neg_\R \top) \vee (\neg_\R \bot)
                }{
                    \infer{
                        \vdash (\neg_\R \bot)
                    }{
                        \infer{
                            \bot \vdash \R
                        }{
                            \infer{
                                \bot \vdash \bot
                            }{
                            }
                        }
                    }
                }
            }
            $$
        \item $A = \bot$.
            $$
            \infer{
                \vdash (\bot \vee \neg \bot)^{\neg_\R}
            }{
                \infer{
                    \vdash (\bot \Rightarrow \R) \vee (\neg_\R \top)
                }{
                    \infer{
                        \vdash (\neg_\R \bot)
                    }{
                        \infer{
                            \bot \vdash \R
                        }{
                            \infer{\bot \vdash \bot}{}
                        }
                    }
                }
            }
            $$

        \item $A = (a \dot{=} b)$.

            $$
            \infer{
                (\Pi_3) :\:\vdash (a \dot{=} b) \vee (\neg_\R(a \dot{=} b))
            }{
                \infer{
                    \vdash (a \dot{=} b) \vee (\neg(a \dot{=} b))
                }{
                    \text{decidability of QF formulas}
                }
                &
                \infer{
                    (a \dot{=} b) \vdash (a \dot{=} b)
                }{
                }
                &
                \infer{
                    \neg(a \dot{=} b) \vdash \neg_\R(a \dot{=} b)
                }{
                    \Psi_1
                }
            }
            $$

            $$
            \infer{
                \vdash ((a \dot{=} b) \vee \neg(a \dot{=} b))^{\neg_\R}
            }{
                \infer{
                    \vdash \neg_\R\neg_\R(a \dot{=} b) \vee (\neg_\R\neg_\R\neg_\R(a \dot{=} b))
                }{
                    \infer{
                        (a \dot{=} b) \vdash \neg_\R\neg_\R(a \dot{=} b) \vee (\neg_\R\neg_\R\neg_\R(a \dot{=} b))
                    }{
                        \infer{
                            (a \dot{=} b) \vdash \neg_\R\neg_\R(a \dot{=} b)
                        }{
                            \Psi_2
                        }
                    }&
                    \infer{
                        \neg_\R(a \dot{=} b) \vdash \neg_\R\neg_\R(a \dot{=} b) \vee (\neg_\R\neg_\R\neg_\R(a \dot{=} b))
                    }{
                        \infer{
                            \neg_\R(a \dot{=} b) \vdash \neg_\R\neg_\R\neg_\R(a \dot{=} b)
                        }{
                            \Psi_2
                        }
                    }&
                    \Pi_3
                }
            }
            $$
        \item $A = B \vee C$
        
            $IH_B : \; \vdash (B \vee \neg B)^{\neg_\R}$
            
            $IH_C : \; \vdash (C \vee \neg C)^{\neg_\R}$

            $$
            \infer{
                (\Pi_6) : {\neg_\R} B^{\neg_\R}, {\neg_\R} C^{\neg_\R}, (B^{\neg_\R} \vee C^{\neg_\R}) \vdash \R
            }{
                    \infer{B^{\neg_\R} \vee C^{\neg_\R} \vdash B^{\neg_\R} \vee C^{\neg_\R}
                }{
                }&
                \infer{
                    {\neg_\R} B^{\neg_\R}, {\neg_\R} C^{\neg_\R}, B^{\neg_\R} \vdash \R
                }{
                    \infer{
                        {\neg_\R} B^{\neg_\R}, {\neg_\R} C^{\neg_\R}, B^{\neg_\R} \vdash B^{\neg_\R}
                    }{
                    }
                }&
                \infer{
                    {\neg_\R} B^{\neg_\R}, {\neg_\R} C^{\neg_\R}, C^{\neg_\R} \vdash \R
                }{
                    \infer{
                        {\neg_\R} B^{\neg_\R}, {\neg_\R} C^{\neg_\R}, C^{\neg_\R} \vdash C^{\neg_\R}
                    }{
                    }
                }
            }
            $$
            
            $$
                \infer{
                    (\Pi_7) : {\neg_\R} B^{\neg_\R}, {\neg_\R} C^{\neg_\R} \vdash {\neg_\R}{\neg_\R}(B^{\neg_\R} \vee C^{\neg_\R}) \vee {\neg_\R}{\neg_\R}{\neg_\R} (B^{\neg_\R} \vee C^{\neg_\R})
                }{
                    \infer{
                        {\neg_\R} B^{\neg_\R}, {\neg_\R} C^{\neg_\R} \vdash {\neg_\R}{\neg_\R}{\neg_\R} (B^{\neg_\R} \vee C^{\neg_\R})
                    }{
                        \infer{
                            {\neg_\R} B^{\neg_\R}, {\neg_\R} C^{\neg_\R}, {\neg_\R}{\neg_\R} (B^{\neg_\R} \vee C^{\neg_\R}) \vdash \R
                        }{
                            \infer{
                                {\neg_\R} B^{\neg_\R}, {\neg_\R} C^{\neg_\R} \vdash {\neg_\R} (B^{\neg_\R} \vee C^{\neg_\R})
                            }{
                                \infer{
                                    {\neg_\R} B^{\neg_\R}, {\neg_\R} C^{\neg_\R}, (B^{\neg_\R} \vee C^{\neg_\R}) \vdash \R
                                }{
                                    \Pi_6
                                }
                            }
                        }
                    }
                }
            $$

            $$
            \infer{
                (\Pi_8) : {\neg_\R} B^{\neg_\R} \vdash {\neg_\R}{\neg_\R}(B^{\neg_\R} \vee C^{\neg_\R}) \vee {\neg_\R}{\neg_\R}{\neg_\R} (B^{\neg_\R} \vee C^{\neg_\R})
            }{
                \infer{
                    \vdash (C \vee {\neg_\R} C)
                }{
                        \infer{\vdash (C \vee \neg C)^{\neg_\R}
                    }{
                    }
                }&
                \infer{
                    {\neg_\R} B^{\neg_\R}, C^{\neg_\R} \vdash {\neg_\R}{\neg_\R}(B^{\neg_\R} \vee C^{\neg_\R}) \vee {\neg_\R}{\neg_\R}{\neg_\R} (B^{\neg_\R} \vee C^{\neg_\R}
                }{
                    \infer{
                        {\neg_\R} B^{\neg_\R}, C^{\neg_\R} \vdash {\neg_\R}{\neg_\R}(B^{\neg_\R} \vee C^{\neg_\R})
                    }{
                        \infer
                        {
                            \Psi_3
                        }{
                            \infer{
                                {\neg_\R} B^{\neg_\R}, C^{\neg_\R}, {\neg_\R}(B^{\neg_\R} \vee C^{\neg_\R})\vdash (B^{\neg_\R} \vee C^{\neg_\R})
                            }{
                                \infer{
                                    {\neg_\R} B^{\neg_\R}, C^{\neg_\R}, {\neg_\R}(B^{\neg_\R} \vee C^{\neg_\R})\vdash C^{\neg_\R})
                                }{
                                }
                            }
                        }
                    }
                }&
                \Pi_7
            }
            $$
            
            $$
                    \infer{
                        (\Pi_9) : {\neg_\R} B^{\neg_\R} \vdash {\neg_\R}{\neg_\R}(B^{\neg_\R} \vee C^{\neg_\R}) \vee {\neg_\R}{\neg_\R}{\neg_\R} (B^{\neg_\R} \vee C^{\neg_\R})
                    }{
                        \Pi_8
                    }
            $$

            $$
            \infer{
                \vdash (B \vee C)^{\neg_\R} \vee ({\neg_\R} (B \vee C)^{\neg_\R})
            }{
                \infer{
                    \vdash {\neg_\R}{\neg_\R}(B^{\neg_\R} \vee C^{\neg_\R}) \vee {\neg_\R}{\neg_\R}{\neg_\R} (B^{\neg_\R} \vee C^{\neg_\R})
                }{
                    \infer{
                        \vdash B^{\neg_\R} \vee \neg B^{\neg_\R}
                    }{
                        \infer{
                            \vdash (B \vee {\neg_\R} B)^{\neg_\R}
                        }{
                        }
                    }&
                    \infer{
                        B^{\neg_\R} \vdash {\neg_\R}{\neg_\R}(B^{\neg_\R} \vee C^{\neg_\R}) \vee {\neg_\R}{\neg_\R}{\neg_\R} (B^{\neg_\R} \vee C^{\neg_\R})
                    }{
                        \infer{
                            B^{\neg_\R} \vdash {\neg_\R}{\neg_\R}(B^{\neg_\R} \vee C^{\neg_\R})
                        }{
                            \infer{
                                \Psi_3
                            }{
                                \infer{
                                    B^{\neg_\R}, {\neg_\R}(B^{\neg_\R} \vee C^{\neg_\R}) \vdash B^{\neg_\R} \vee C^{\neg_\R}
                                }{
                                    \infer{
                                        B^{\neg_\R}, {\neg_\R}(B^{\neg_\R} \vee C^{\neg_\R}) \vdash B^{\neg_\R}
                                    }{
                                    }
                                }
                            }
                        }
                    }&
                    \Pi_9
                }
            }
            $$

        \item $A = B \wedge C$
        
            $(IH_B) : \; \vdash (B \vee \neg B)^{\neg_\R}$
            
            $(IH_C) : \; \vdash (C \vee \neg C)^{\neg_\R}$


            $$
                \infer{
                    (\Pi_4) : B^{\neg_\R}, \neg_\R C^{\neg_\R} \vdash (B^{\neg_\R} \wedge C^{\neg_\R}) \vee \neg_\R(B^{\neg_\R} \wedge C^{\neg_\R})
                }{
                    \infer{
                        B^{\neg_\R}, \neg C^{\neg_\R} \vdash \neg_\R(B^{\neg_\R} \wedge C^{\neg_\R})
                    }{
                        \infer{
                            B^{\neg_\R}, \neg C^{\neg_\R}, B^{\neg_\R} \wedge C^{\neg_\R} \vdash \R
                        }{
                            \infer{
                                B^{\neg_\R}, B^{\neg_\R} \wedge C^{\neg_\R} \vdash C^{\neg_\R}
                            }{
                                \infer{
                                    B^{\neg_\R}, B^{\neg_\R} \wedge C^{\neg_\R} \vdash B^{\neg_\R} \wedge C^{\neg_\R}
                                }{
                                }
                            }
                        }
                    }
                }
            $$


            $$
            \infer{
                \Pi_5 : B^{\neg_\R} \vdash (B^{\neg_\R} \wedge C^{\neg_\R}) \vee \neg_\R(B^{\neg_\R} \wedge C^{\neg_\R})
            }{
                \infer{
                    \vdash (C^{\neg_\R} \vee \neg_\R C^{\neg_\R})
                }{
                    \infer{
                        \vdash (C \vee \neg C)^{\neg_\R}
                    }{
                        IH_C
                    }
                }&
                \infer{
                    B^{\neg_\R}, C^{\neg_\R} \vdash (B^{\neg_\R} \wedge C^{\neg_\R}) \vee \neg_\R(B^{\neg_\R} \wedge C^{\neg_\R})
                }{
                    \infer{
                        B^{\neg_\R}, C^{\neg_\R} \vdash B^{\neg_\R} \wedge C^{\neg_\R}
                    }{
                        \infer{
                            B^{\neg_\R}, C^{\neg_\R} \vdash B^{\neg_\R}
                        }{
                        }&
                        \infer{
                            B^{\neg_\R}, C^{\neg_\R} \vdash C^{\neg_\R}
                        }{
                        }
                    }
                }&
                \Pi_4
            }
            $$

            $$
            \infer{
                \vdash ((B \wedge C) \vee \neg(B \wedge C))^{\neg_\R}
            }{\infer{\Psi_3}{
                    \infer{\vdash (B^{\neg_\R} \wedge C^{\neg_\R}) \vee {\neg_\R}(B^{\neg_\R} \wedge C^{\neg_\R})
                }{
                        \infer{\vdash B^{\neg_\R} \vee {\neg_\R} B^{\neg_\R}
                    }{
                            \infer{\vdash (B \vee \neg B)^{\neg_\R}
                        }{
                            IH_B
                        }
                    }
                    &
                        \infer{B^{\neg_\R} \vdash (B^{\neg_\R} \wedge C^{\neg_\R}) \vee {\neg_\R}(B^{\neg_\R} \wedge C^{\neg_\R})
                    }{
                        \Pi_5
                    }
                    &
                    \infer{
                        \neg B^{\neg_\R} \vdash (B^{\neg_\R} \wedge C^{\neg_\R}) \vee {\neg_\R}(B^{\neg_\R} \wedge C^{\neg_\R})
                    }{
                        \infer{
                            \neg B^{\neg_\R} \vdash {\neg_\R}(B^{\neg_\R} \wedge C^{\neg_\R})
                        }{
                            \infer{
                                \neg B^{\neg_\R}, B^{\neg_\R} \wedge C^{\neg_\R} \vdash \R
                            }{
                                \infer{
                                    B^{\neg_\R} \wedge C^{\neg_\R} \vdash B^{\neg_\R}
                                }{
                                    \infer{
                                        B^{\neg_\R} \wedge C^{\neg_\R} \vdash B^{\neg_\R} \wedge C^{\neg_\R}
                                    }{
                                    }
                                }
                            }
                        }
                    }
                }
            }}
            $$
        \item $A = B \Rightarrow C$
        
            $(IH_B) : \; \vdash (B \vee \neg B)^{\neg_\R}$
            
            $(IH_C) : \; \vdash (C \vee \neg C)^{\neg_\R}$
            
            $$
            $$
    \end{itemize}

    \item We proof this property by induction on $A$ and we denote by $IH$ the induction hypothesis.
    \begin{itemize}
        \item $A=\bottom$
            $$
                \infer{
                    \R \vdash \R
                }{
                }
            $$
        \item $A=\top$
            $$
                \infer{
                    \R \vdash \top
                }{
                }
            $$
        \item $A=(a \dot{=} b)$
            $$
                \infer{
                    \R \vdash (a \dot{=} b)^{\neg_\R}
                }{
                    \infer{
                        \R, \neg_\R(a \dot{=} b) \vdash \R
                    }{
                    }
                }
            $$
        \item $A=B\wedge C$
            $$
                \infer{
                    \R \vdash B^\ngr \wedge C^\ngr
                }{
                    \infer{
                        \R \vdash B^\ngr
                    }{
                        IH
                    }&
                    \infer{
                        \R \vdash C^\ngr
                    }{
                        IH
                    }
                }
            $$
        \item $A=B \Rightarrow C$
            $$
                \infer{
                    \R \vdash B^\ngr \Rightarrow C^\ngr
                }{
                    \infer{
                        \R, B^\ngr \vdash C^\ngr
                    }{
                        IH
                    }
                }
            $$
        \item $A=B \vee C$
            $$
                \infer{
                    \R \vdash \ngr\ngr(B^\ngr \vee C^\ngr)
                }{
                    \infer{
                        \R, \ngr(B^\ngr \vee C^\ngr) \vdash \R
                    }{
                    }
                }
            $$
        \item $A=\forall x B$
            $$
                \infer{
                    \R \vdash \forall x B^\ngr
                }{
                    \infer{
                        \R \vdash B^\ngr
                    }{
                        IH
                    }
                }
            $$
        \item $A=\exists x B$
            $$
                \infer{
                    \R \vdash \ngr\ngr(\exists x B^\ngr)
                }{
                    \infer{
                        \R, \ngr(\exists x B^\ngr) \vdash \R
                    }{
                    }
                }
            $$
    \end{itemize}
    So, $\R\vdash A^{\neg_\R}$
    
    \item We proof this property by induction on $A$ and we denote by $IH$ the induction hypothesis.
    \begin{itemize}
        \item $A=\bottom$
            $$
                \infer{
                    \neg_\R\neg_\R \bottom^{\neg_\R} \vdash \bottom^{\neg_\R}
                }{
                    \infer{
                        \neg_\R\neg_\R \R \vdash \R
                    }{
                        \infer{
                            \neg_\R\neg_\R \R \vdash \R\Rightarrow\R\Rightarrow\R
                        }{
                        }&
                        \infer{
                            \neg_\R\neg_\R \R \vdash \R\Rightarrow\R
                        }{
                            \infer{
                                \neg_\R\neg_\R \R, \R \vdash \R
                            }{
                            }
                        }
                    }
                }
            $$
        \item $A=\top$
            $$
                \infer{
                    \neg_\R\neg_\R \top^{\neg_\R} \vdash \top^{\neg_\R}
                }{
                    \infer{
                        \neg_\R\neg_\R \top^{\neg_\R} \vdash \top
                    }{
                    }
                }
            $$
        \item $A=(a \dot{=} b)$
            $$
            \infer{
                                (\Theta_1) : \neg_\R \neg_\R (a \dot{=} b)^{\neg_\R}, \neg_\R(a \dot{=} b), \neg_\R \neg_\R (a \dot{=} b) \vdash \R
                            }{
                                \infer{
                                    \neg_\R \neg_\R (a \dot{=} b)^{\neg_\R}, \neg_\R(a \dot{=} b), \neg_\R \neg_\R (a \dot{=} b) \vdash \neg_\R \neg_\R (a \dot{=} b)
                                }{
                                }&
                                \infer{
                                    \neg_\R(a \dot{=} b), \neg_\R \neg_\R (a \dot{=} b) \vdash \neg_\R (a \dot{=} b)
                                }{
                                }
                            }
            $$
            
            $$
                \infer{
                    \neg_\R \neg_\R (a \dot{=} b)^{\neg_\R} \vdash (a \dot{=} b)^{\neg_\R}
                }{
                    \infer{
                        \neg_\R \neg_\R (a \dot{=} b)^{\neg_\R}, \neg_\R(a \dot{=} b) \vdash \R
                    }{
                        \infer{
                            \neg_\R \neg_\R (a \dot{=} b)^{\neg_\R}, \neg_\R(a \dot{=} b) \vdash \neg_\R \neg_\R \neg_\R \neg_\R (a \dot{=} b)
                        }{
                        }&
                        \infer{
                            \neg_\R \neg_\R (a \dot{=} b)^{\neg_\R}, \neg_\R(a \dot{=} b) \vdash \neg_\R \neg_\R \neg_\R (a \dot{=} b)
                        }{
                            \Theta_1
                        }
                    }
                }
            $$
        \item $A=B\wedge C$
        
            $$
            \infer{
                            (\Theta_2) : \neg_\R\neg_\R(B \wedge C)^{\neg_\R}, \neg_\R B^{\neg_\R} \vdash \neg_\R(B \wedge C)^{\neg_\R}
                        }{
                            \infer{
                                \neg_\R\neg_\R(B \wedge C)^{\neg_\R}, \neg_\R B^{\neg_\R}, (B \wedge C)^{\neg_\R} \vdash \R
                            }{
                                \infer{
                                    \neg_\R\neg_\R(B \wedge C)^{\neg_\R}, \neg_\R B^{\neg_\R}, (B \wedge C)^{\neg_\R} \vdash \neg_\R B^{\neg_\R}
                                }{
                                }&
                                \infer{
                                    \neg_\R\neg_\R(B \wedge C)^{\neg_\R}, \neg_\R B^{\neg_\R}, (B \wedge C)^{\neg_\R} \vdash B^{\neg_\R}
                                }{
                                    \infer{
                                        \neg_\R\neg_\R(B \wedge C)^{\neg_\R}, \neg_\R B^{\neg_\R}, (B \wedge C)^{\neg_\R} \vdash B^{\neg_\R} \wedge C^{\neg_\R}
                                    }{
                                    }
                                }
                            }
                        }
            $$        
        
            $$
            \infer{
                    (\Theta_3) : \neg_\R\neg_\R(B \wedge C)^{\neg_\R} \vdash \neg_\R\neg_\R B^{\neg_\R}
                }{
                    \infer{
                        \neg_\R\neg_\R(B \wedge C)^{\neg_\R}, \neg_\R B^{\neg_\R} \vdash \R
                    }{
                        \infer{
                            \neg_\R\neg_\R(B \wedge C)^{\neg_\R}, \neg_\R B^{\neg_\R} \vdash \neg_\R\neg_\R(B \wedge C)^{\neg_\R}
                        }{
                        }&
                        \Theta_2
                    }
                }
            $$        
        
            $$
            \infer{
                (\Theta_4) : \neg_\R\neg_\R(B \wedge C)^{\neg_\R} \vdash B^{\neg_\R}
            }{
                \Theta_3
                &
                \infer{
                    \neg_\R\neg_\R(B \wedge C)^{\neg_\R} \vdash \neg_\R\neg_\R B^{\neg_\R} \Rightarrow  B^{\neg_\R}
                }{
                    \infer{
                        \neg_\R\neg_\R(B \wedge C)^{\neg_\R}, \neg_\R\neg_\R B^{\neg_\R} \vdash  B^{\neg_\R}
                    }{
                        IH_B
                    }
                }
            }
            $$
            
            $$
            \infer{
                            (\Theta_5) : \neg_\R\neg_\R(B \wedge C)^{\neg_\R}, \neg_\R C^{\neg_\R} \vdash \neg_\R(B \wedge C)^{\neg_\R}
                        }{
                            \infer{
                                \neg_\R\neg_\R(B \wedge C)^{\neg_\R}, \neg_\R C^{\neg_\R}, (B \wedge C)^{\neg_\R} \vdash \R
                            }{
                                \infer{
                                    \neg_\R\neg_\R(B \wedge C)^{\neg_\R}, \neg_\R C^{\neg_\R}, (B \wedge C)^{\neg_\R} \vdash \neg_\R C^{\neg_\R}
                                }{
                                }&
                                \infer{
                                    \neg_\R\neg_\R(B \wedge C)^{\neg_\R}, \neg_\R C^{\neg_\R}, (B \wedge C)^{\neg_\R} \vdash C^{\neg_\R}
                                }{
                                    \infer{
                                        \neg_\R\neg_\R(B \wedge C)^{\neg_\R}, \neg_\R C^{\neg_\R}, (B \wedge C)^{\neg_\R} \vdash B^{\neg_\R} \wedge C^{\neg_\R}
                                    }{
                                    }
                                }
                            }
                        }
            $$        
        
            $$
            \infer{
                    (\Theta_6) : \neg_\R\neg_\R(B \wedge C)^{\neg_\R} \vdash \neg_\R\neg_\R C^{\neg_\R}
                }{
                    \infer{
                        \neg_\R\neg_\R(B \wedge C)^{\neg_\R}, \neg_\R C^{\neg_\R} \vdash \R
                    }{
                        \infer{
                            \neg_\R\neg_\R(B \wedge C)^{\neg_\R}, \neg_\R C^{\neg_\R} \vdash \neg_\R\neg_\R(B \wedge C)^{\neg_\R}
                        }{
                        }&
                        \Theta_5
                    }
                }
            $$        
        
            $$
            \infer{
                (\Theta_7) : \neg_\R\neg_\R(B \wedge C)^{\neg_\R} \vdash C^{\neg_\R}
            }{
                \Theta_6
                &
                \infer{
                    \neg_\R\neg_\R(B \wedge C)^{\neg_\R} \vdash \neg_\R\neg_\R C^{\neg_\R} \Rightarrow  C^{\neg_\R}
                }{
                    \infer{
                        \neg_\R\neg_\R(B \wedge C)^{\neg_\R}, \neg_\R\neg_\R C^{\neg_\R} \vdash  C^{\neg_\R}
                    }{
                        IH_C
                    }
                }
            }
            $$
            
            $$
                \infer{
                    \neg_\R\neg_\R(B \wedge C)^{\neg_\R} \vdash (B \wedge C)^{\neg_\R}
                }{
                    \infer{
                        \neg_\R\neg_\R(B \wedge C)^{\neg_\R} \vdash B^{\neg_\R} \wedge C^{\neg_\R}
                    }{
                        \Theta_4
                        &
                        \Theta_7
                    }
                }
            $$
        \item $A=B \Rightarrow C$
            $$
                \infer{
                    \neg_\R\neg_\R (B \Rightarrow C)^{\neg_\R} \vdash (B \Rightarrow C)^{\neg_\R}
                }{
                    \infer{
                        \neg_\R\neg_\R (B \Rightarrow C)^{\neg_\R} \vdash B^{\neg_\R} \Rightarrow C^{\neg_\R}
                    }{
                        \infer{
                            \neg_\R\neg_\R (B \Rightarrow C)^{\neg_\R}, B^{\neg_\R} \vdash C^{\neg_\R}
                        }{
                            todo
                        }
                    }
                }
            $$
        \item $A=B \vee C$
            $$            
                    \infer{
                        (\Theta_8) : \neg_\R\neg_\R(B \vee C)^{\neg_\R}, \neg_\R(B^{\neg_\R} \vee C^{\neg_\R}), (B \vee C)^{\neg_\R} \vdash \neg_\R(B^{\neg_\R} \vee C^{\neg_\R})
                    }{
                        \infer{
                            \neg_\R\neg_\R(B \vee C)^{\neg_\R}, \neg_\R(B^{\neg_\R} \vee C^{\neg_\R}), (B \vee C)^{\neg_\R}, B^{\neg_\R} \vee C^{\neg_\R} \vdash \R
                        }{
                            \infer{
                                \neg_\R(B^{\neg_\R} \vee C^{\neg_\R}) \vdash \neg_\R(B^{\neg_\R} \vee C^{\neg_\R})
                            }{
                            }&
                            \infer{
                                B^{\neg_\R} \vee C^{\neg_\R} \vdash B^{\neg_\R} \vee C^{\neg_\R}
                            }{
                            }
                        }
                    }
            $$
            
            $$
            \infer{
                (\Theta_9) : \neg_\R\neg_\R(B \vee C)^{\neg_\R}, \neg_\R(B^{\neg_\R} \vee C^{\neg_\R}) \vdash \neg_\R(B \vee C)^{\neg_\R}
            }{
                \infer{
                    \neg_\R\neg_\R(B \vee C)^{\neg_\R}, \neg_\R(B^{\neg_\R} \vee C^{\neg_\R}), (B \vee C)^{\neg_\R} \vdash \R
                }{
                    \infer{
                        \neg_\R\neg_\R(B^{\neg_\R} \vee C^{\neg_\R}) \vdash \neg_\R\neg_\R(B^{\neg_\R} \vee C^{\neg_\R})
                    }{
                    }&
                    \Theta_8
                }
            }
            $$
        
            $$
                \infer{
                    \neg_\R\neg_\R(B \vee C)^{\neg_\R} \vdash (B \vee C)^{\neg_\R}
                }{
                    \infer{
                        \neg_\R\neg_\R(B \vee C)^{\neg_\R} \vdash \neg_\R\neg_\R(B^{\neg_\R} \vee C^{\neg_\R})
                    }{
                        \infer{
                            \neg_\R\neg_\R(B \vee C)^{\neg_\R}, \neg_\R(B^{\neg_\R} \vee C^{\neg_\R}) \vdash \R
                        }{
                            \infer{
                                \neg_\R\neg_\R(B \vee C)^{\neg_\R}, \neg_\R(B^{\neg_\R} \vee C^{\neg_\R}) \vdash \neg_\R\neg_\R(B \vee C)^{\neg_\R}
                            }{
                            }&
                            \Theta_9
                        }
                    }
                }
            $$
        \item $A=\forall x B$
            $$
                \infer{
                    \neg_\R\neg_\R \forall x B^{\neg_\R} \vdash \forall x B^{\neg_\R}
                }{
                    \infer{
                       \neg_\R\neg_\R \forall x B^{\neg_\R} \vdash B^{\neg_\R}
                    }{
                        IH
                    }
                }
            $$
        \item $A=\exists x B$
            $$\infer{
                            (\Theta_{10}) : \neg_\R\neg_\R(\exists x B)^{\neg_\R}, \neg_\R(\exists x B^{\neg_\R}) \vdash \neg_\R(\exists x B)^{\neg_\R}
                        }{
                            \infer{
                                \neg_\R\neg_\R(\exists x B)^{\neg_\R}, \neg_\R(\exists x B^{\neg_\R}), (\exists x B)^{\neg_\R} \vdash \R
                            }{
                                \infer{
                                    (\exists x B)^{\neg_\R} \vdash \neg_\R\neg_\R\exists x B^{\neg_\R}
                                }{
                                }&
                                \infer{
                                    \neg_\R(\exists x B^{\neg_\R}), (\exists x B)^{\neg_\R} \vdash \neg_\R\exists x B^{\neg_\R}
                                }{
                                    \infer{
                                        \neg_\R(\exists x B^{\neg_\R}), (\exists x B)^{\neg_\R}, \exists x B^{\neg_\R} \vdash \R
                                    }{
                                        \infer{
                                            \neg_\R(\exists x B^{\neg_\R}) \vdash \neg_\R(\exists x B^{\neg_\R})
                                        }{
                                        }&
                                        \infer{
                                            \exists x B^{\neg_\R} \vdash \exists x B^{\neg_\R}
                                        }{
                                        }
                                    }
                                }
                            }
                        }
            $$
        
            $$
                \infer{
                    \neg_\R\neg_\R(\exists x B)^{\neg_\R} \vdash \neg_\R\neg_\R(\exists x B^{\neg_\R})
                }{
                    \infer{
                        \neg_\R\neg_\R(\exists x B)^{\neg_\R}, \neg_\R(\exists x B^{\neg_\R}) \vdash \R
                    }{
                        \infer{
                            \neg_\R\neg_\R(\exists x B)^{\neg_\R} \vdash \neg_\R\neg_\R(\exists x B)^{\neg_\R}
                        }{
                        }&
                        \Theta_{10}
                    }
                }
            $$
    \end{itemize}
    So, $\neg_\R\neg_\R A^{\neg_\R}\vdash A^{\neg_\R}$
\end{enumerate}