\begin{enumerate}
    \item Injectivity of $S$
    $$    
                                \infer{
                                    (\Xi_1) : \neg_\R\neg_\R S(x)\dot{=}S(y), \neg_\R x\dot{=}y, S(x)\dot{=}S(y)  \vdash x\dot{=}y
                                }{
                                    \infer{
                                        \neg_\R\neg_\R S(x)\dot{=}S(y), \neg_\R x\dot{=}y, S(x)\dot{=}S(y)  \vdash S(x)\dot{=}S(y) 
                                    }{
                                    }&
                                    \infer{
                                        \vdash S(x)\dot{=}S(y) \Rightarrow x\dot{=}y
                                    }{
                                    }
                                }
    $$
    
    
    $$
    \infer{
                            (\Xi_2) : \neg_\R\neg_\R S(x)\dot{=}S(y), \neg_\R x\dot{=}y \vdash \neg_\R S(x)\dot{=}S(y) 
                        }{
                            \infer{
                                \neg_\R\neg_\R S(x)\dot{=}S(y), \neg_\R x\dot{=}y, S(x)\dot{=}S(y)  \vdash\R 
                            }{
                                \infer{
                                    \neg_\R\neg_\R S(x)\dot{=}S(y), \neg_\R x\dot{=}y, S(x)\dot{=}S(y)  \vdash\neg_\R x\dot{=}y
                                }{
                                }&
                                \Xi_1
                            }
                        }
    $$    
    
    $$
    \infer{
        \vdash (\forall xy (S(x)\dot{=}S(y) \Rightarrow x\dot{=}y))^{\neg_\R}
    }{
        \infer{
            \vdash \forall xy (\neg_\R\neg_\R S(x)\dot{=}S(y) \Rightarrow \neg_\R\neg_\R x\dot{=}y)
        }{
            \infer{
                \vdash \neg_\R\neg_\R S(x)\dot{=}S(y) \Rightarrow \neg_\R\neg_\R x\dot{=}y
            }{
                \infer{
                    \neg_\R\neg_\R S(x)\dot{=}S(y) \vdash\neg_\R\neg_\R x\dot{=}y
                }{
                    \infer{
                        \neg_\R\neg_\R S(x)\dot{=}S(y), \neg_\R x\dot{=}y \vdash \R 
                    }{
                        \infer{
                            \neg_\R\neg_\R S(x)\dot{=}S(y) \vdash \neg_\R\neg_\R S(x)\dot{=}S(y) 
                        }{
                        }&
                        \Xi_2
                    }
                }
            }
        }
    }
    $$
    
    \item Non confusion
    
    $$
    \infer{
        \vdash (\forall x \neg S(x)\dot{=}0)^{\neg_\R}
    }{
        \infer{
            \vdash \forall x \neg_\R\neg_\R\neg_\R S(x)\dot{=}0
        }{
            \infer{
                \vdash \neg_\R\neg_\R\neg_\R S(x)\dot{=}0
            }{
                \infer{
                    \neg_\R\neg_\R S(x)\dot{=}0 \vdash \R
                }{
                   \infer{
                        \neg_\R\neg_\R S(x)\dot{=}0 \vdash \neg_\R\neg_\R S(x)\dot{=}0
                    }{
                    }&
                   \infer{
                        \neg_\R\neg_\R S(x)\dot{=}0 \vdash \neg_\R S(x)\dot{=}0
                    }{
                        \infer{
                           \neg_\R\neg_\R S(x)\dot{=}0, S(x)\dot{=}0\vdash \R 
                        }{
                            \infer{
                                \neg_\R\neg_\R S(x)\dot{=}0, S(x)\dot{=}0\vdash \bottom 
                            }{
                                \infer{
                                    \neg_\R\neg_\R S(x)\dot{=}0, S(x)\dot{=}0\vdash S(x)\dot{=}0\ 
                                }{   
                                }&
                                \infer{
                                    \vdash \neg S(x)\dot{=}0\ 
                                }{
                                    \infer{
                                        \vdash \neg \forall xS(x)\dot{=}0\ 
                                    }{
                                    }
                                }
                            }
                        }
                    }
                }
            }
        }
    }
    $$
    
    \item Induction Scheme
    
    $$
    \infer{
        (\Xi_3) : A[0/x]^{\neg_\R}, \forall y(A[y/x]^{\neg_\R} \Rightarrow A[S(y)/x]^{\neg_\R}) \vdash \forall y(A[y/x]^{\neg_\R} \Rightarrow A[S(y)/x]^{\neg_\R}) \Rightarrow A^{\neg_\R}
    }{
        \infer{
            \vdash A[0/x]^{\neg_\R} \Rightarrow \forall y(A[y/x]^{\neg_\R} \Rightarrow A[S(y)/x]^{\neg_\R}) \Rightarrow A^{\neg_\R}
        }{
        }&
        \infer{
            A[0/x]^{\neg_\R} \vdash A[0/x]^{\neg_\R}
        }{
        }
    }
    $$
    
    $$
    \infer{
        \vdash (A[0/x] \Rightarrow \forall y(A[y/x] \Rightarrow A[S(y)/x]) \Rightarrow \forall x A)^{\neg_\R}
    }{
        \infer{
            \vdash A[0/x]^{\neg_\R} \Rightarrow \forall y(A[y/x]^{\neg_\R} \Rightarrow A[S(y)/x]^{\neg_\R}) \Rightarrow \forall x A^{\neg_\R}
        }{
            \infer{
                A[0/x]^{\neg_\R} \vdash \forall y(A[y/x]^{\neg_\R} \Rightarrow A[S(y)/x]^{\neg_\R}) \Rightarrow \forall x A^{\neg_\R}
            }{
                \infer{
                    A[0/x]^{\neg_\R}, \forall y(A[y/x]^{\neg_\R} \Rightarrow A[S(y)/x]^{\neg_\R}) \vdash \forall x A^{\neg_\R}
                }{
                    \infer{
                        A[0/x]^{\neg_\R}, \forall y(A[y/x]^{\neg_\R} \Rightarrow A[S(y)/x]^{\neg_\R}) \vdash A^{\neg_\R}
                    }{
                        \Xi_3
                        &
                        \infer{
                            \forall y(A[y/x]^{\neg_\R} \Rightarrow A[S(y)/x]^{\neg_\R}) \vdash \forall y(A[y/x]^{\neg_\R} \Rightarrow A[S(y)/x]^{\neg_\R})
                        }{
                        }
                    }
                }
            }
        }
    }
    $$
\end{enumerate}